Fin de la première preuve !

src/int63/CnfInt63.v
@@ -63,171 +63,267 @@ Section Checker.
     | a::b::c => a::(clean c)
     end.
 
-(*TODO : remplace egalité booléène par equivalent*)
- Definition check_BuildDefInt lits :=
-  let n := PArray.length lits in
-  if (n == Int63Op.digits + 1)&&(Lit.is_pos (lits.[0]))
-  then (
-    match get_form (Lit.blit (lits.[0])) with
-    | Fatom a => 
-      match get_atom a with
-      | Abop b h1 h2 => 
-        match (b,get_atom h1,get_atom h2) with
-        | (BO_eq Tint,Acop (CO_int x),Acop (CO_int y)) => 
-          let test_correct i0 l :=
-            if i0 == 0
-            then Lit.is_pos l
-            else (
+  Definition check_BuildDefInt lits :=
+    let n := PArray.length lits in
+    if (n == Int63Op.digits + 1)&&(Lit.is_pos (lits.[0]))
+    then (
+      match get_form (Lit.blit (lits.[0])) with
+      | Fatom a => 
+        match get_atom a with
+        | Abop b h1 h2 => 
+          match (b,get_atom h1,get_atom h2) with
+          | (BO_eq Tint,Acop (CO_int x),Acop (CO_int y)) => 
+            let test_correct i0 l :=
+              if i0 == 0
+              then Lit.is_pos l
+              else (
+                match get_form (Lit.blit l) with
+                | Fiff l1 l2 =>
+                  match (get_form (Lit.blit l1),get_form (Lit.blit l2)) with
+                  | (Fatom a1,Fatom a2) =>
+                    match (get_atom a1,get_atom a2) with
+                    | (Auop (UO_index j) hx1,Auop (UO_index k) hy1) => 
+                      match (get_atom hx1,get_atom hy1) with
+                      | (Acop (CO_int x1),Acop (CO_int y1)) => (Lit.is_pos l1)&&(Lit.is_pos l2)&&(negb (Lit.is_pos l))&&(j == i0-1)&&(k == j)&&(x == x1)&&(y==y1)
+                      | _ => false
+                      end
+                    | _ => false
+                    end
+                  | _ => false
+                  end
+                | _ => false
+                end
+                   )
+            in
+            if forallbi (fun i l => test_correct i l) lits
+            then PArray.to_list lits
+            else C._true
+          | _ => C._true
+          end
+        | _ => C._true
+        end
+      | _ => C._true
+      end
+         )
+    else C._true
+  .
+
+
+  Definition check_BuildProjInt lits i :=
+    let n := PArray.length lits in
+    if (n == Int63Op.digits + 1)&&(i < Int63Op.digits)
+    then (
+      match get_form (Lit.blit (lits.[0])) with
+      | Fatom a => 
+        match get_atom a with
+        | Abop b h1 h2 => 
+          match (b,get_atom h1,get_atom h2) with
+          | (BO_eq t,Acop (CO_int x),Acop (CO_int y)) => 
+            let test_correct i0 l :=
               match get_form (Lit.blit l) with
               | Fiff l1 l2 =>
                 match (get_form (Lit.blit l1),get_form (Lit.blit l2)) with
                 | (Fatom a1,Fatom a2) =>
                   match (get_atom a1,get_atom a2) with
-                  | (Auop (UO_index x1) j,Auop (UO_index y1) k) => (negb (Lit.is_pos l1))&&(negb (Lit.is_pos l2))&&(j == i0-1)&&(k == j)&&(x == x1)&&(y==y1)
+                  | (Auop (UO_index j) hx1,Auop (UO_index k) hy1) => 
+                    match (get_atom hx1,get_atom hy1) with
+                    | (Acop (CO_int x1),Acop (CO_int y1)) => (Lit.is_pos l1)&&(Lit.is_pos l2)&&(negb (Lit.is_pos (lits.[0])))&&(Lit.is_pos l)&&(Typ.eqb t Typ.Tint)&&(j == i0)&&(k == j)&&(x == x1)&&(y==y1)
+                    | _ => false
+                    end
+
                   | _ => false
                   end
                 | _ => false
                 end
               | _ => false
-              end
-                 )
-          in
-          if forallbi (fun i l => test_correct i l) lits
-          then PArray.to_list lits
-          else C._true
+              end            
+            in
+            if test_correct i (lits.[i+1]) 
+            then (lits.[i+1])::(lits.[0])::nil
+            else C._true
+          | _ => C._true
+          end
         | _ => C._true
         end
       | _ => C._true
       end
-    | _ => C._true
-    end
-       )
-  else C._true
+         )
+    else C._true
   .
 
+(*
+Section Proof.
 
-Definition check_BuildProjInt lits i :=
-  let n := PArray.length lits in
-  if (n == Int63Op.digits + 1)&&(i < Int63Op.digits)
-  then (
-    match get_form (Lit.blit (lits.[0])) with
-    | Fatom a => 
-      match get_atom a with
-      | Abop b h1 h2 => 
-        match (b,get_atom h1,get_atom h2) with
-        | (BO_eq t,Acop (CO_int x),Acop (CO_int y)) => 
-          let test_correct i0 l :=
-            match get_form (Lit.blit l) with
-            | Fiff l1 l2 =>
-              match (get_form (Lit.blit l1),get_form (Lit.blit l2)) with
-              | (Fatom a1,Fatom a2) =>
-                match (get_atom a1,get_atom a2) with
-                | (Auop (UO_index x1) j,Auop (UO_index y1) k) => (negb (Lit.is_pos (lits.[0])))&&(Lit.is_pos l1)&&(Lit.is_pos l2)&&(Typ.eqb t Typ.Tint)&&(j == i0)&&(k == j)&&(x == x1)&&(y==y1)
-                | _ => false
-                end
-              | _ => false
-              end
-            | _ => false
-            end            
-          in
-          if test_correct i (lits.[i+1]) 
-          then (lits.[i+1])::(lits.[0])::nil
-          else C._true
-        | _ => C._true
-        end
-      | _ => C._true
-      end
-    | _ => C._true
-    end
-       )
-  else C._true
-  .
+    Variables (t_i : array typ_eqb)
+              (t_func : array (Atom.tval t_i))
+              (ch_atom : Atom.check_atom t_atom)
+              (ch_form : Form.check_form t_form)
+              (wt_t_atom : Atom.wt t_i t_func t_atom).
 
+    Local Notation check_atom :=
+      (check_aux t_i t_func (get_type t_i t_func t_atom)).
 
+    Local Notation interp_form_hatom :=
+      (Atom.interp_form_hatom t_i t_func t_atom).
 
+    Local Notation rho :=
+      (Form.interp_state_var interp_form_hatom t_form).
 
-Variable interp_hatom : hatom -> bool.
+    Local Notation t_interp := (t_interp t_i t_func t_atom).
 
-Local Notation rho := (Form.interp_state_var interp_hatom t_form).
+    Local Notation interp_atom :=
+      (interp_aux t_i t_func (get t_interp)).
 
-Hypothesis Hch_f : check_form t_form.
+    Let wf_t_atom : Atom.wf t_atom.
+    Proof. destruct (Atom.check_atom_correct _ ch_atom); auto. Qed.
 
-Check rho.
+    Let def_t_atom : default t_atom = Atom.Acop Atom.CO_xH.
+    Proof. destruct (Atom.check_atom_correct _ ch_atom); auto. Qed.
 
-Let Hwfrho : Valuation.wf rho.
+    Let def_t_form : default t_form = Form.Ftrue.
+    Proof.
+      destruct (Form.check_form_correct interp_form_hatom _ ch_form) as [H _]; destruct H; auto.
+    Qed.
+
+    Let wf_t_form : Form.wf t_form.
+    Proof.
+      destruct (Form.check_form_correct interp_form_hatom _ ch_form) as [H _]; destruct H; auto.
+    Qed.
+
+    Let wf_rho : Valuation.wf rho.
+    Proof.
+      destruct (Form.check_form_correct interp_form_hatom _ ch_form); auto.
+    Qed.
+*)
+
+  Section Proof.
+    
+    Variables (t_i : array typ_eqb)
+              (t_func : array (Atom.tval t_i))
+              (ch_atom : Atom.check_atom t_atom)
+              (ch_form : Form.check_form t_form)
+              (wt_t_atom : Atom.wt t_i t_func t_atom).
+
+    Local Notation check_atom :=
+      (check_aux t_i t_func (get_type t_i t_func t_atom)).
+
+    Local Notation interp_form_hatom :=
+      (Atom.interp_form_hatom t_i t_func t_atom).
+
+    Local Notation rho :=
+      (Form.interp_state_var interp_form_hatom t_form).
+
+    Local Notation t_interp := (t_interp t_i t_func t_atom).
+
+    Local Notation interp_atom :=   
+      (interp_aux t_i t_func (get t_interp)).
+      Check interp_atom.
+      Check interp_form_hatom.
+
+    Let wf_t_atom : Atom.wf t_atom.
+    Proof. destruct (Atom.check_atom_correct _ ch_atom); auto. Qed.
+
+    Let def_t_atom : default t_atom = Atom.Acop Atom.CO_xH.
+    Proof. destruct (Atom.check_atom_correct _ ch_atom); auto. Qed.
+
+    Let def_t_form : default t_form = Form.Ftrue.
+    Proof.
+      destruct (Form.check_form_correct interp_form_hatom _ ch_form) as [H _]; destruct H; auto.
+    Qed.
+
+    Let wf_t_form : Form.wf t_form.
+    Proof.
+      destruct (Form.check_form_correct interp_form_hatom _ ch_form) as [H _]; destruct H; auto.
+    Qed.
+
+    Let wf_rho : Valuation.wf rho.
+    Proof.
+      destruct (Form.check_form_correct interp_form_hatom _ ch_form); auto.
+    Qed.
+
+  Lemma lit_interp_true : Lit.interp rho Lit._true = true.
   Proof.
-    destruct (check_form_correct interp_hatom _ Hch_f) as (_, H);exact H. 
+    apply Lit.interp_true.
+    apply wf_rho.
   Qed.
 
 
-Lemma lit_interp_true : Lit.interp rho Lit._true = true.
-  apply Lit.interp_true.
-  apply Hwfrho.
-Qed.
-
-
-Let rho_interp : forall x : int,
-    rho x = Form.interp interp_hatom t_form (t_form.[ x]).
+  Let rho_interp : forall x : int, rho x = Form.interp interp_form_hatom t_form (t_form.[ x]).
   Proof.
-    destruct (check_form_correct interp_hatom _ Hch_f) as ((H,H0), _).
+    destruct (check_form_correct interp_form_hatom _ ch_form) as ((H,H0), _).
     intros x;apply wf_interp_form;trivial.
   Qed.
 
-Lemma bool_impl : forall a b, (b = true -> a = true) -> a = true \/ b = false.
-Proof.
-intros.
-destruct a.
-left.
-trivial.
-right.
-destruct b.
-symmetry.
-apply H.
-trivial.
-trivial.
-Qed.
-
-Lemma lit_interp_impl : forall a b rho,(Lit.interp rho b = true -> Lit.interp rho a = true) -> (Lit.interp rho a =true \/Lit.interp rho (Lit.neg b) = true).
-Proof.
-  intros.
-  rewrite (Lit.interp_neg rho b).
-  rewrite negb_true_iff.
-  apply bool_impl.
-  apply H.
-Qed.
-
-
-Lemma valid_check_BuildProjInt : forall lits i, C.valid rho (check_BuildProjInt lits i).
+  Lemma bool_impl : forall a b, (b = true -> a = true) -> a = true \/ b = false.
   Proof.
-   unfold check_BuildProjInt,C.valid;intros lits i.
-   case_eq ((length lits == digits + 1) && (i < digits)).
-
-   intros. case_eq (t_form.[Lit.blit (lits.[0])]).
-   intros. case_eq (t_atom.[i0]);intros; auto using C.interp_true.
-   case_eq b;intros; auto using C.interp_true.
-   case_eq (t_atom.[i1]);intros; auto using C.interp_true.
-   case_eq c;intros; auto using C.interp_true.
-   case_eq (t_atom.[i2]);intros; auto using C.interp_true.
-   case_eq c0;intros; auto using C.interp_true.
-   case_eq (t_form.[Lit.blit (lits.[i+1])]);intros;auto using C.interp_true.
-   case_eq (t_form.[Lit.blit i5]);intros;auto using C.interp_true.
-   case_eq (t_form.[Lit.blit i6]);intros;auto using C.interp_true.
-   case_eq (t_atom.[i7]);intros;auto using C.interp_true.
-   case_eq u;intros;auto using C.interp_true.
-   case_eq (t_atom.[i8]);intros;auto using C.interp_true.
-   case_eq u0;intros;auto using C.interp_true.
-   case_eq (negb (Lit.is_pos (lits .[ 0])) && Lit.is_pos i5 && Lit.is_pos i6 && Typ.eqb t Typ.Tint && (i9 == i) && (i11 == i9) && (i3 == i10) && (i4 == i12));intros;case_eq (Lit.is_pos (lits.[i+1]));intros.
-   apply andb_true_iff in H14; destruct H14;apply andb_true_iff in H14; destruct H14;apply andb_true_iff in H14; destruct H14;apply andb_true_iff in H14; destruct H14;apply andb_true_iff in H14; destruct H14;apply andb_true_iff in H14; destruct H14;apply andb_true_iff in H14; destruct H14.
-   simpl; rewrite orb_false_r; apply orb_true_iff. 
-
-   unfold Lit.interp; unfold Var.interp; rewrite rho_interp; rewrite H15; rewrite H7; rewrite negb_true_iff in H14; rewrite H14; rewrite negb_true_iff; apply bool_impl; intro.
-   unfold Form.interp; unfold Form.interp_aux; unfold Lit.interp; unfold Var.interp; rewrite H22; rewrite H21; rewrite rho_interp; rewrite H8;rewrite rho_interp; rewrite H9; unfold Form.interp; unfold Form.interp_aux; unfold Form.interp;unfold Form.interp_aux. 
-   rewrite rho_interp in H23; rewrite H0 in H23; unfold Form.interp in H23; unfold Form.interp_aux in H23.
-
-
-
-  intros; auto using C.interp_true;intros; auto using C.interp_true;intros; auto using C.interp_true;intros; auto using C.interp_true;intros; auto using C.interp_true;intros; auto using C.interp_true;intros; auto using C.interp_true;intros; auto using C.interp_true;intros; auto using C.interp_true;intros; auto using C.interp_true;intros; auto using C.interp_true;intros; auto using C.interp_true.
+    intros;destruct a;
+    [(left;trivial) | (right;destruct b;[(symmetry;apply H;trivial) | trivial])].
   Qed.
- 
 
+  Lemma lit_interp_impl : forall a b rho,(Lit.interp rho b = true -> Lit.interp rho a = true) -> (Lit.interp rho a =true \/Lit.interp rho (Lit.neg b) = true).
+  Proof.
+    intros;rewrite (Lit.interp_neg rho b);rewrite negb_true_iff;apply bool_impl;apply H.
+  Qed.
+
+
+  Lemma valid_check_BuildProjInt : forall lits i, C.valid rho (check_BuildProjInt lits i).
+  Proof.
+    unfold check_BuildProjInt,C.valid. intros lits i.
+    case_eq ((length lits == digits + 1) && (i < digits)).
+
+    intros. case_eq (t_form.[Lit.blit (lits.[0])]).
+    intros. case_eq (t_atom.[i0]);intros; auto using C.interp_true.
+    case_eq b;intros; auto using C.interp_true.
+    case_eq (t_atom.[i1]);intros; auto using C.interp_true.
+    case_eq c;intros; auto using C.interp_true.
+    case_eq (t_atom.[i2]);intros; auto using C.interp_true.
+    case_eq c0;intros; auto using C.interp_true.
+    case_eq (t_form.[Lit.blit (lits.[i+1])]);intros;auto using C.interp_true.
+    case_eq (t_form.[Lit.blit i5]);intros;auto using C.interp_true.
+    case_eq (t_form.[Lit.blit i6]);intros;auto using C.interp_true.
+    case_eq (t_atom.[i7]);intros;auto using C.interp_true.
+    case_eq u;intros;auto using C.interp_true.
+    case_eq (t_atom.[i8]);intros;auto using C.interp_true.
+    case_eq u0;intros;auto using C.interp_true.
+    case_eq (t_atom.[i9]);intros;auto using C.interp_true.
+    case_eq c1;intros;auto using C.interp_true.
+    case_eq (t_atom.[i11]);intros;auto using C.interp_true.
+    case_eq c2;intros;auto using C.interp_true.
+    case_eq (Lit.is_pos i5 && Lit.is_pos i6 && negb (Lit.is_pos (lits .[ 0])) && Lit.is_pos (lits .[ i + 1]) && Typ.eqb t Typ.Tint && (i10 == i) && (i12 == i10) && (i3 == i13) && (i4 == i14));intros.
+    apply andb_true_iff in H18; destruct H18;apply andb_true_iff in H18; destruct H18;apply andb_true_iff in H18; destruct H18;apply andb_true_iff in H18; destruct H18;apply andb_true_iff in H18; destruct H18;apply andb_true_iff in H18; destruct H18;apply andb_true_iff in H18; destruct H18;apply andb_true_iff in H18; destruct H18.
+    
+    rewrite Int63Properties.eqb_spec in H19; rewrite Int63Properties.eqb_spec in H20; rewrite Int63Properties.eqb_spec in H21; rewrite Int63Properties.eqb_spec in H22;apply Typ.eqb_spec in H23;subst i10; subst i12; subst i13; subst i14.
+    symmetry in H11;symmetry in H4; symmetry in H6; rewrite H4 in H15; rewrite H6 in H17; rewrite H11 in H13;subst u0;subst t; subst c1; subst c2;symmetry in H11;symmetry in H4; symmetry in H6.
+    rewrite negb_true_iff in H25.
+
+    simpl; rewrite orb_false_r; apply orb_true_iff.
+    unfold Lit.interp; rewrite H24; rewrite H25; rewrite negb_true_iff; unfold Var.interp; rewrite !rho_interp; rewrite H7; rewrite H0.
+    simpl; unfold Lit.interp; rewrite H18; rewrite H26; unfold Var.interp; rewrite !rho_interp; rewrite H8; rewrite H9;simpl.
+    unfold Atom.interp_form_hatom; unfold interp_hatom; rewrite !t_interp_wf. 
+    rewrite H1; rewrite H10;rewrite H12; simpl; rewrite !t_interp_wf.
+    unfold interp_uop; unfold interp_bop; rewrite H11; rewrite H2; simpl; rewrite H3;rewrite H5;rewrite H14;rewrite H16; simpl; unfold interp_cop; rewrite H4;rewrite H6;simpl.
+    apply bool_impl; intro H27; apply Int63Properties.eqb_spec in H27; subst i4; trivial; apply Bool.eqb_true_iff; trivial.
+
+    apply wf_t_atom. apply def_t_atom. 
+    apply wf_t_atom. apply def_t_atom.
+    apply wf_t_atom. apply def_t_atom.
+    apply wf_t_atom. apply def_t_atom.
+    apply wf_t_atom. apply def_t_atom.
+    apply wf_t_atom. apply def_t_atom.
+    apply wf_t_atom. apply def_t_atom. 
+    auto using C.interp_true.
+    intros; auto using C.interp_true.
+    intros; auto using C.interp_true.
+    intros; auto using C.interp_true.
+    intros; auto using C.interp_true.
+    intros; auto using C.interp_true.
+    intros; auto using C.interp_true.
+    intros; auto using C.interp_true.
+    intros; auto using C.interp_true.
+    intros; auto using C.interp_true.
+    intros; auto using C.interp_true.
+  Qed.
+
+  End Proof.
+  
 End Checker.
